src/Sound/VCGen/Sound.dfy
@@ -69,6 +69,64 @@ module VCGenOmni {
           }
         }
       }
+    case Call(proc, args) =>
+      var Pre := SeqSubstitute(proc.Pre, args.ToExpr());
+      var Post := SeqSubstitute(proc.Post, args.ToExpr());
+      VCs := seq(|Pre|, (i: nat) requires i < |Pre| => 
+        SeqExprDepthLemma(Pre, Pre[i]);
+        context_in.MkEntailment(Pre[i]));
+      var vNew, context' := context_in.AddVarSet(args.OutArgs()) by {
+        args.OutArgsDepthLemma();
+      }
+      context := context'.AddSeq(Post) by {
+        forall post <- Post { SeqExprDepthLemma(Post, post); }
+      }
+      if (forall e <- VCs :: e.Holds()) {
+        forall st: State | context_in.IsSatisfiedOn(st)
+          ensures Omni.SemSingle(s, context_in.AdjustState(st), context.AdjustedModels) {
+          forall v <- args.OutArgs() 
+            ensures v < |context_in.AdjustState(st)| {
+            args.OutArgsDepthLemma();
+          }
+          forall e <- Pre 
+            ensures e.IsDefinedOn(|context_in.AdjustState(st)|) 
+            ensures context_in.AdjustState(st).Eval(e) 
+          {
+            SeqExprDepthLemma(Pre, e);
+            assert context_in.MkEntailment(e).Holds() by {
+              context_in.MkEntailmentSeqLemma(Pre, e) by {
+                forall e <- Pre { SeqExprDepthLemma(Pre, e); }
+              }
+            }
+            EvalConjLemma(context_in.ctx, st);
+            context_in.AdjustStateSubstituteLemma(st, e);
+          }
+          forall st': State | 
+            && st' in context_in.AdjustState(st).EqExcept(args.OutArgs())
+            && (forall e <- Post :: e.IsDefinedOn(|st'|) && st'.Eval(e))
+            ensures st' in context.AdjustedModels {
+            var st'' := st.UpdateMapShift(vNew, map i: Idx | i in args.OutArgs() :: st'[i]);
+            assert st' == context.AdjustState(st'') by {
+              assert (map i: Idx | i in args.OutArgs() :: st'[i]).Keys == args.OutArgs();
+            }
+            assert context.IsSatisfiedOn(st'') by {
+              assert forall i <- context.incarnation :: i < |st''|;
+              forall e <- context.ctx
+                ensures e.IsDefinedOn(|st''|)
+                ensures st''.Eval(e) {
+                if e in context_in.ctx {
+                  e.EvalDepthLemma(st, st'');
+                } else {
+                  assert e in context'.SeqSubstitute(Post);
+                  var e' := context'.GetSeqSubstituteLemma(Post, e);
+                  context'.SubstituteIsDefinedOnLemma(e', |st''|);
+                  context'.AdjustStateSubstituteLemma(st'', e');
+                }
+              }
+            }
+          }
+        }
+      }
   }
 
   ghost function BlockWPSeq(bcont: Block.Continuation, post: iset<State>) : Omni.Continuation
@@ -319,7 +377,7 @@ module VCGenOmni {
           if (forall e <- VCs :: e.Holds()) {
             forall st: State | context.IsSatisfiedOn(st)
               ensures Omni.SeqSem([Loop(inv, body)] + cont, context.AdjustState(st), BlockWPSeq(bcont, AllStates)) {
-              var inv' := inv.Sem() * AssignmentTarget.EqsTo(assnvars, context.AdjustState(st));
+              var inv' := inv.Sem() * context.AdjustState(st).EqExcept(assnvars);
               var st' := context.AdjustState(st);
               Omni.SemLoopWithCont(inv, body, cont, st', BlockWPSeq(bcont, AllStates), inv') by {
                 assert st' in inv.Sem() by {
